Aiur/Circuit.lean
@@ -2,3 +2,4 @@ import Aiur.Circuit.Basic
 import Aiur.Circuit.Compile
 import Aiur.Circuit.Derivation
 import Aiur.Circuit.MemoDerivation
+import Aiur.Circuit.MemoAcyclic
